before policy change

reinvent/naturelle.v
@@ -16,6 +16,9 @@ Inductive ou (A B : Prop) : Prop :=
 Inductive egale (A : Type) (x : A) : A -> Prop :=
 | egreflexion : egale A x x.
 
+Axiom fonc_egalite: forall (A: Type) (B: A -> Type) (f g: forall x:A, B x),
+  (forall x: A, egale _ (f x) (g x)) -> egale _ f g.
+
 Definition fegale (A B : Type) (f : A -> B) (x y : A) (H : egale _ x y) :=
   match H in (egale _ _ a) return (egale _ (f x) (f a)) with
   | egreflexion _ _ => egreflexion _ (f x)
@@ -35,6 +38,8 @@ apply Hxy.
 Qed.
 
 Definition nepas := fun A : Prop => A -> Faux.
+
+Definition ssi (A B: Prop) := et (A -> B) (B -> A).
 
 
 (*===== Booleen =====*)
@@ -312,7 +317,12 @@ Definition neufNdix (H : egale _ neuf dix) :=
 
 (* ===== Ensemble ===== *)
 
-Definition Ensemble (M: Type) := M -> Prop.
+(* Definition Ensemble (M: Type) := M -> Prop. *)
+Record Ensemble := _Ensemble {
+  Sorte: Type;
+  avoir: Sorte -> Prop
+}.
+
 Definition ensemble (M: egtaper) := sorte M -> booleenne.
 
 Lemma axiom_ensemble : forall (M: egtaper) (A: ensemble M), 
@@ -322,12 +332,14 @@ Proof.
   case (A x); apply identite.
 Qed.
 
-Axiom Axiom_Ensemble : forall (T: Type) (A: Ensemble T),
-  forall (x: T), ou (A x) (nepas (A x)).
+Axiom Axiom_Ensemble : forall (A: Ensemble),
+  forall (x: Sorte A), ou (avoir A x) (nepas (avoir A x)).
 
-Definition VideEnsemble (T: Type): Ensemble T := fun _ => Faux.
-Definition MemeEnsemble (T: Type): Ensemble T := fun _ => Vraie.
-Definition SousEnsemble (T: Type) (A B: Ensemble T)
+Definition VideEnsemble (T: Type) := _Ensemble T (fun _ => Faux).
+Definition MemeEnsemble (T: Type) := _Ensemble T (fun _ => Vraie).
+Record SousEnsMelange (A: Ensemble) := _SousEnsMelange {
+  
+}
   := forall (x: T), A x -> B x.
 
 Definition appartenir (M: egtaper) (x: sorte M) (ens: ensemble M) := estvraie (ens x).
@@ -337,9 +349,26 @@ Definition memeensemble (M: egtaper): ensemble M := fun _ => vraie.
 
 Definition sousensemble (M: egtaper) (A B: ensemble M)
   := forall (x: sorte M), appartenir _ x A -> appartenir _ x B.
+  
+Record Cartographie := _Cartographie {
+  Tdom: Type;
+  Tcod: Type;
+  Domaine: Ensemble Tdom;
+  Codomaine: Ensemble Tcod;
+  Fonc: Tdom -> Tcod;
+  Fermer_fonc : forall (x: Tdom), Domaine x -> Codomaine (Fonc x)
+}.
+
+Definition Injection (f: Cartographie)
+  := forall (x y: Tdom f), Domaine _ x -> Domaine _ y -> egale _ (Fonc f x) (Fonc f y) -> egale _ x y.
+
+Definition Surjection (f: Cartographie)
+  := forall (x: Tcod f), exists x': Tdom f, egale _ x (Fonc f x').
+
+Definition Bijection (f: Cartographie) := et (Injection f) (Surjection f).
 
 (* ===== Group ===== *)
-
+(* 
 Record groupe: Type := _groupe {
   porteur: egtaper;
   support: ensemble porteur;
@@ -385,112 +414,127 @@ Definition homomorphisme (G H: groupe) (f: gtaper H -> gtaper G) :=
 
 
 Definition noyau (G H: groupe) (f: gtaper H -> gtaper G) : ensemble (porteur H) :=
-  fun x => gegop _ (elemid G) (f x).
+  fun x => gegop _ (elemid G) (f x). *)
 
 (* Definition image (G H: groupe) (f: gtaper H -> gtaper G) : ensemble (porteur G) := *)
 
 
 Record Groupe: Type := _Groupe {
-  Porteur: Type;
-  Support: Ensemble Porteur;
-  Operatrice: Porteur -> Porteur -> Porteur;
-  Inverse: Porteur -> Porteur;
-  Elemid: Porteur;
-  Fermer_ope: forall (x y: Porteur), 
-    Support x -> Support y -> Support (Operatrice x y);
-  Fermer_inv: forall (x: Porteur),
-    Support x -> Support (Inverse x);
-  Fermer_id: Support Elemid;
-  Assoc_ope: forall (x y z: Porteur),
-    Support x -> Support y -> Support z
-    -> egale _ (Operatrice (Operatrice x y) z) (Operatrice x (Operatrice y z));
-  Inv_gauche: forall (x: Porteur),
-    Support x -> egale _ Elemid (Operatrice (Inverse x) x);
-  Inv_droite: forall (x: Porteur),
-    Support x -> egale _ Elemid (Operatrice x (Inverse x));
-  Id_droite: forall (x: Porteur),
-    Support x -> egale _ x (Operatrice x Elemid)
+  Tsupp: Type;
+  Supp: Ensemble Tsupp;
+  Ope: Tsupp -> Tsupp -> Tsupp;
+  Inv: Tsupp -> Tsupp;
+  Id: Tsupp;
+  Fermer_ope: forall (x y: Tsupp), 
+    Supp x -> Supp y -> Supp (Ope x y);
+  Fermer_inv: forall (x: Tsupp),
+    Supp x -> Supp (Inv x);
+  Fermer_id: Supp Id;
+  Assoc_ope: forall (x y z: Tsupp),
+    Supp x -> Supp y -> Supp z
+    -> egale _ (Ope x (Ope y z)) (Ope (Ope x y) z);
+  Inv_gauche: forall (x: Tsupp),
+    Supp x -> egale _ Id (Ope (Inv x) x);
+  Inv_droite: forall (x: Tsupp),
+    Supp x -> egale _ Id (Ope x (Inv x));
+  Id_droite: forall (x: Tsupp),
+    Supp x -> egale _ x (Ope x Id)
 }.
 
-Lemma Id_gauche: forall (G: Groupe) (x: Porteur G),
-  (Support G) x -> egale _ x (Operatrice _ (Elemid G) x).
+Lemma Id_gauche: forall (G: Groupe) (x: Tsupp G),
+  (Supp G) x -> egale _ x (Ope _ (Id G) x).
 Proof.
   intros G x H.
   case (egsym _ _ _ (Inv_droite G x H)).
-  case (egsym _ _ _ (Assoc_ope _ x (Inverse _ x) x H (Fermer_inv _ x H) H)).
+  case (Assoc_ope _ x (Inv _ x) x H (Fermer_inv _ x H) H).
   case (Inv_gauche G x H).
   case (Id_droite G x H).
   apply egreflexion.
 Qed.
 
-Lemma Reduire_gauche: forall (G: Groupe) (x y z: Porteur G), 
-  (Support G) x -> (Support G) y -> (Support G) z
-  -> egale _ (Operatrice _ x y) (Operatrice _ x z)
+Lemma Reduire_gauche: forall (G: Groupe) (x y z: Tsupp G), 
+  (Supp G) x -> (Supp G) y -> (Supp G) z
+  -> egale _ (Ope _ x y) (Ope _ x z)
   -> egale _ y z.
 Proof.
   intros G x y z Gx Gy Gz Hxyxz.
   case (egsym _ _ _(Id_gauche _ y Gy)).
   case (egsym _ _ _(Id_gauche _ z Gz)).
   case (egsym _ _ _ (Inv_gauche _ x Gx)).
-  case (egsym _ _ _ (Assoc_ope _ (Inverse _ x) x y (Fermer_inv _ x Gx) Gx Gy)).
-  case (egsym _ _ _ (Assoc_ope _ (Inverse _ x) x z (Fermer_inv _ x Gx) Gx Gz)).
+  case (Assoc_ope _ (Inv _ x) x y (Fermer_inv _ x Gx) Gx Gy).
+  case (Assoc_ope _ (Inv _ x) x z (Fermer_inv _ x Gx) Gx Gz).
   apply fegale, Hxyxz.
 Qed.
 
-Lemma Transpo_gauche: forall (G: Groupe) (x y z: Porteur G),
-  (Support G) x -> (Support G) y -> (Support G) z
-  -> egale _ (Operatrice _ x y) z -> egale _ y (Operatrice _ (Inverse _ x) z).
+Lemma Transpo_gauche: forall (G: Groupe) (x y z: Tsupp G),
+  (Supp G) x -> (Supp G) y -> (Supp G) z
+  -> egale _ (Ope _ y x) z -> egale _ x (Ope _ (Inv _ y) z).
 Proof.
-  intros G x y z Gx Gy Gz H0.
+  intros G y x z Gy Gx Gz H0.
   case (egsym _ _ _ (Id_gauche _ y Gy)).
   case (egsym _ _ _ (Inv_gauche _ x Gx)).
-  case (egsym _ _ _ (Assoc_ope _ (Inverse _ x) x y (Fermer_inv _ x Gx) Gx Gy)).
+  case (Assoc_ope _ (Inv _ x) x y (Fermer_inv _ x Gx) Gx Gy).
   apply fegale, H0.
 Qed.
 
-Lemma InvInv: forall (G: Groupe) (x: Porteur G),
-  (Support G) x -> egale _ x (Inverse _ (Inverse _ x)).
+Lemma Invdinv_ident: forall (G: Groupe) (x: Tsupp G),
+  (Supp G) x -> egale _ x (Inv _ (Inv _ x)).
 Proof.
   intros G x Gx.
   pose (Fermer_inv _ x Gx) as Ginvx.
-  apply (Reduire_gauche _ (Inverse _ x) x (Inverse _ (Inverse _ x)) Ginvx Gx (Fermer_inv _ (Inverse _ x) Ginvx)).
+  case (Reduire_gauche _ (Inv _ x) x (Inv _ (Inv _ x)) Ginvx Gx (Fermer_inv _ (Inv _ x) Ginvx)).
   case (Inv_gauche _ x Gx).
-  case (Inv_droite _ (Inverse _ x) Ginvx).
+  case (Inv_droite _ (Inv _ x) Ginvx).
+  apply egreflexion.
+  apply egreflexion.
+Qed.
+
+Lemma Invope_opeinvinv: forall (G: Groupe) (x y: Tsupp G),
+  (Supp G) x -> (Supp G) y -> egale _ (Inv _ (Ope _ x y)) (Ope _ (Inv _ y) (Inv _ x)).
+Proof.
+  intros G x y Gx Gy.
+  pose (Fermer_inv _ _ (Fermer_ope _ _ _ Gx Gy)) as Ginvxy.
+  apply (Transpo_gauche _ _ _ _ Ginvxy Gy (Fermer_inv _ _ Gx)).
+  case (egsym _ _ _(Id_droite _ _ (Fermer_inv _ _ Gx))).
+  apply (Transpo_gauche _ _ _ _ (Fermer_ope _ _ _ Gy Ginvxy) Gx (Fermer_id _)).
+  case (egsym _ _ _ (Assoc_ope _ _ _ _ Gx Gy Ginvxy)).
+  case (Inv_droite _ _ (Fermer_ope _ _ _ Gx Gy)).
+  apply egreflexion.
+Qed.
+
+Lemma Id_invid: forall (G: Groupe), egale _ (Id G) (Inv _ (Id _)).
+Proof.
+  intros G.
+  case (egsym _ _ _ (Id_droite G _ (Fermer_inv _ _ (Fermer_id _)))).
+  apply (Transpo_gauche _ _ _ _ (Fermer_id _) (Fermer_id _) (Fermer_id _)).
+  case (Id_droite _ _ (Fermer_id G)).
   apply egreflexion.
 Qed.
 
 
-Definition cartographie (T1 T2: Type) (A: Ensemble T1) (B: Ensemble T2)
-  (f: T1 -> T2) := forall (x: T1), A x -> B (f x).
+Definition Homomorphisme (G H: Groupe) 
+  := forall x y: Tsupp H, Supp H x -> Supp H y -> egale _ (f (Ope H x y)) (Ope G (f x) (f y))).
 
-Definition injection (T1 T2: Type) (A: Ensemble T1) (B: Ensemble T2)
-  (f: T1 -> T2)
-  := (cartographie _ _ A B f) -> forall x y: T1, A x -> A y -> egale _ (f x) (f y) -> egale _ x y.
-
-Definition Homomorphisme (G H: Groupe) (f: Porteur H -> Porteur G) 
-  := et (cartographie _ _ (Support H) (Support G) f)
-   (forall x y: Porteur H, egale _ (f (Operatrice H x y)) (Operatrice G (f x) (f y))).
-
-Theorem Hom_preserve_id: forall (G H: Groupe) (f: Porteur H -> Porteur G),
-  Homomorphisme _ _ f -> egale _ (Elemid G) (f (Elemid H)).
+Theorem Hom_preserve_id: forall (G H: Groupe) (f: Tsupp H -> Tsupp G),
+  Homomorphisme _ _ f -> egale _ (Id G) (f (Id H)).
 Proof.
   intros G H f _Hhom.
   unfold Homomorphisme in _Hhom.
   case _Hhom.
   intros Hcart Hhom.
   unfold cartographie in Hcart.
-  case (egsym _ _ _ (Inv_gauche _ (f (Elemid H)) (Hcart (Elemid H) (Fermer_id H)))).
+  case (egsym _ _ _ (Inv_gauche _ (f (Id H)) (Hcart (Id H) (Fermer_id H)))).
   apply egsym.
-  pose (Hcart (Elemid H) (Fermer_id H)) as Gfe.
-  apply (Transpo_gauche _ (f (Elemid H)) (f (Elemid H)) (f (Elemid H)) Gfe Gfe Gfe).
-  case (Hhom (Elemid H) (Elemid H)).
-  case (Id_droite _ (Elemid H) (Fermer_id H)).
+  pose (Hcart (Id H) (Fermer_id H)) as Gfe.
+  apply (Transpo_gauche _ (f (Id H)) (f (Id H)) (f (Id H)) Gfe Gfe Gfe).
+  case (Hhom (Id H) (Id H) (Fermer_id _) (Fermer_id _)).
+  case (Id_droite _ (Id H) (Fermer_id H)).
   apply egreflexion.
 Qed.
 
-Theorem Hom_preserve_inv: forall (G H: Groupe) (f: Porteur H -> Porteur G),
+Theorem Hom_preserve_inv: forall (G H: Groupe) (f: Tsupp H -> Tsupp G),
   Homomorphisme _ _ f -> 
-  forall (x: Porteur H), (Support H) x -> egale _ (f (Inverse _ x)) (Inverse _ (f x)).
+  forall (x: Tsupp H), (Supp H) x -> egale _ (f (Inv _ x)) (Inv _ (f x)).
 Proof.
   intros G H f _Hhom.
   case _Hhom.
@@ -498,30 +542,264 @@ Proof.
   intros x Hx.
   unfold cartographie in Hcart.
   pose (Fermer_inv _ (f x) (Hcart x Hx)) as Ginvfx.
-  case (egsym _ _ _ (Id_droite _ (Inverse _ (f x)) Ginvfx)).
-  apply (Transpo_gauche _ _ _ _ (Hcart x Hx) (Hcart (Inverse _ x) (Fermer_inv _ x Hx)) (Fermer_id _)).
-  case Hhom.
+  case (egsym _ _ _ (Id_droite _ (Inv _ (f x)) Ginvfx)).
+  apply (Transpo_gauche _ _ _ _ (Hcart x Hx) (Hcart (Inv _ x) (Fermer_inv _ x Hx)) (Fermer_id _)).
+  case (Hhom _ _ Hx (Fermer_inv _ _ Hx)).
   case (Inv_droite _ _ Hx).
   apply (egsym _ _ _ (Hom_preserve_id _ _ f _Hhom)).
 Qed.
 
-Definition SousGroupe (G: Groupe) (Hsupp: Ensemble (Porteur G))
-  (HsousG: SousEnsemble _ Hsupp (Support G))
-  (HFermer_ope: forall (x y: Porteur G), Hsupp x -> Hsupp y -> Hsupp (Operatrice G x y))
-  (HFermer_inv: forall (x: Porteur G), Hsupp x -> Hsupp (Inverse G x))
-  (HFermer_id: Hsupp (Elemid G))
+Record SousGroupeMelange (G: Groupe): Type := _SousGroupeMelange {
+  Hsupp: Ensemble (Tsupp G);
+  HsousG : SousEnsemble _ Hsupp (Supp G);
+  HFermer_ope: forall (x y: Tsupp G), Hsupp x -> Hsupp y -> Hsupp (Ope G x y);
+  HFermer_inv: forall (x: Tsupp G), Hsupp x -> Hsupp (Inv G x);
+  HFermer_id: Hsupp (Id G)
+}.
+
+Definition SousGroupe (G: Groupe) (H: SousGroupeMelange G)
+  := _Groupe (Tsupp G) (Hsupp G H) (Ope G) (Inv G) (Id G)
+  (HFermer_ope _ _) (HFermer_inv _ _) (HFermer_id _ _)
+  (fun (x y z: Tsupp G) (Hx: (Hsupp _ _) x) (Hy: (Hsupp _ _) y) (Hz: (Hsupp _ _) z)
+   => Assoc_ope G x y z ((HsousG _ _) x Hx) ((HsousG _ _) y Hy) ((HsousG _ _) z Hz))
+  (fun (x: Tsupp G) (Hx: (Hsupp _ _) x) => Inv_gauche G x ((HsousG _ _) x Hx))
+  (fun (x: Tsupp G) (Hx: (Hsupp _ _) x) => Inv_droite G x ((HsousG _ _) x Hx))
+  (fun (x: Tsupp G) (Hx: (Hsupp _ _) x) => Id_droite G x ((HsousG _ _) x Hx)).
+
+Record reldequiv := _reldequiv {
+  relsorte: Type;
+  relens: Ensemble relsorte;
+  rel: relsorte -> relsorte -> Prop;
+  loireflexe: forall a: relsorte, relens a -> rel a a;
+  loisymetrie: forall a b: relsorte, relens a -> relens b -> rel a b -> rel b a;
+  loitransitive: forall a b c: relsorte, relens a -> relens b -> relens c -> rel a b -> rel b c -> rel a c
+}.
+
+(* relens の内部について同値関係がwell-definedなら外部がどうなろうと知ったこっちゃないので
+   (rel R) y -> みたいなチェックは省く。そもそも実用上relにチェックが内包されそうだけどね。 *)
+Inductive classdequivs (R: reldequiv): Type :=
+| classdequiv : relsorte R -> classdequivs R.
+
+Definition classdequivCommeEnsemble (R: reldequiv) (Cx: classdequivs R): Ensemble (relsorte _) :=
+  match Cx with
+  | classdequiv _ x => rel R x
+  end.
+
+Axiom classdequiv_egalite: forall (R: reldequiv) (Cx Cy: classdequivs R),
+  (forall a, (relens _ a) -> ssi ((classdequivCommeEnsemble _ Cx) a) ((classdequivCommeEnsemble _ Cy) a)) -> egale _ Cx Cy.
+
+Lemma egale_classdequivs: forall (R: reldequiv) (x y: relsorte R),
+  relens _ x -> relens _ y -> rel _ x y -> egale _ (classdequiv _ x) (classdequiv _ y).
+Proof.
+  intros R x y Rx Ry Rxy.
+  apply classdequiv_egalite.
+  simpl.
+  unfold ssi.
+  intros a Ra.
+  apply conjonction.
+  - intros Rxa. apply (loisymetrie _ _ _ Rx Ry) in Rxy. apply (loitransitive _ _ _ _ Ry Rx Ra Rxy Rxa).
+  - intros Rya. apply (loitransitive _ _ _ _ Rx Ry Ra Rxy Rya).
+Qed.
+
+Definition EnsembleDeQuotient (R: reldequiv) : Ensemble (classdequivs R) :=
+  fun Cx => forall x: relsorte R, (classdequivCommeEnsemble _ Cx) x -> relens _ x.
+
+Definition CosetGaucheRel (G: Groupe) (Hmel: SousGroupeMelange G) :=
+  fun x y => (Hsupp _ Hmel) (Ope G (Inv G x) y).
+
+Lemma CosetGauche_reflexe (G: Groupe) (Hmel: SousGroupeMelange G):
+  forall x: Tsupp G, (Supp G) x -> CosetGaucheRel _ Hmel x x.
+Proof.
+  intros x Gx.
+  unfold CosetGaucheRel.
+  case (Inv_gauche _ _ Gx).
+  apply HFermer_id.
+Qed.
+
+Lemma CosetGauche_symetrie (G: Groupe) (Hmel: SousGroupeMelange G):
+  forall x y: Tsupp G, (Supp G) x -> (Supp G) y -> CosetGaucheRel _ Hmel x y -> CosetGaucheRel _ Hmel y x.
+Proof.
+  unfold CosetGaucheRel.
+  intros x y Gx Gy Hxinvy.
+  case (egsym _ _ _ (InvInv _ _ Gx)).
+  case (OpeInv _ _ _ (Fermer_inv _ _ Gx) Gy).
+  apply HFermer_inv.
+  apply Hxinvy.
+Qed.
+
+Lemma CosetGauche_transitive (G: Groupe) (Hmel: SousGroupeMelange G):
+  forall x y z: Tsupp G, (Supp G) x -> (Supp G) y -> (Supp G) z ->
+  CosetGaucheRel _ Hmel x y -> CosetGaucheRel _ Hmel y z -> CosetGaucheRel _ Hmel x z.
+Proof.
+  unfold CosetGaucheRel.
+  intros x y z Gx Gy Gz Hxinvy Hyinvz.
+  case (egsym _ _ _ (Id_gauche _ _ Gz)).
+  case (egsym _ _ _ (Inv_droite _ _ Gy)).
+  case (egsym _ _ _ (Assoc_ope _ _ _ _ Gy (Fermer_inv _ _ Gy) Gz)).
+  case (Assoc_ope _ _ _ _ (Fermer_inv _ _ Gx) Gy (Fermer_ope _ _ _ (Fermer_inv _ _ Gy) Gz)).
+  apply (HFermer_ope _ _ _ _ Hxinvy Hyinvz).
+Qed.
+
+Definition CosetGaucheRel_est_reldequiv (G: Groupe) (Hmel: SousGroupeMelange G) :=
+  _reldequiv (Tsupp G) (Supp G) (CosetGaucheRel G Hmel)
+  (CosetGauche_reflexe _ _) (CosetGauche_symetrie _ _) (CosetGauche_transitive _ _).
+
+
+Definition SousGroupeNormal (G: Groupe) (Hmel: SousGroupeMelange G) :=
+  forall g h: Tsupp G, Supp _ g -> Hsupp _ Hmel h -> Hsupp _ Hmel (Ope _ (Ope _ g h) (Inv _ g)).
+
+
+
+Definition Noyau (G H: Groupe) (f: Tsupp H -> Tsupp G) : Ensemble (Tsupp H) :=
+  fun x => et (Supp H x) (egale _ (Id G) (f x)).
+
+Lemma SousNoyau: forall (G H: Groupe) (f: Tsupp H -> Tsupp G),
+  SousEnsemble _ (Noyau _ _ f) (Supp H).
+Proof.
+  unfold Noyau, SousEnsemble.
+  intros G H f x Hnoy.
+  case Hnoy. intros Hx _.
+  apply Hx.
+Qed.
+
+Lemma NoyauFermer_ope: forall (G H: Groupe) (f: Tsupp H -> Tsupp G),
+  Homomorphisme _ _ f -> forall x y, Noyau _ _ f x -> Noyau _ _ f y -> Noyau _ _ f (Ope _ x y).
+Proof.
+  unfold Noyau.
+  unfold Homomorphisme.
+  intros G H f _Hhom x y Nx Ny.
+  case _Hhom. intros Hcart Hhom.
+  case Nx as [Hx efx], Ny as [Hy efy].
+  case (egsym _ _ _ (Hhom x y Hx Hy)).
+  case efx, efy.
+  case (Id_droite _ _ (Fermer_id _)).
+  apply conjonction.
+  apply (Fermer_ope _ _ _ Hx Hy).
+  apply egreflexion.
+Qed.
+
+Lemma NoyauFermer_inv: forall (G H: Groupe) (f: Tsupp H -> Tsupp G),
+  Homomorphisme _ _ f -> forall x, Noyau _ _ f x -> Noyau _ _ f (Inv _ x).
+Proof.
+  unfold Noyau.
+  intros G H f _Hhom x Nx.
+  case Nx as [Hx Hefx].
+  case _Hhom; intros Hcart Hhom.
+  case (egsym _ _ _ (Hom_preserve_inv _ _ f _Hhom x Hx)).
+  case (egsym _ _ _ (Id_droite _ _ (Fermer_inv _ _ (Hcart x Hx)))).
+  apply conjonction.
+  apply (Fermer_inv _ _ Hx).
+  apply (Transpo_gauche G _ _ _ (Hcart x Hx) (Fermer_id _) (Fermer_id _)).
+  case (Id_droite _ _ (Hcart x Hx)).
+  case Hefx.
+  apply egreflexion.
+Qed.
+
+Lemma NoyauFermer_id: forall (G H: Groupe) (f: Tsupp H -> Tsupp G),
+  Homomorphisme _ _ f -> Noyau _ _ f (Id H).
+Proof.
+  intros G H f _Hhom.
+  case _Hhom.
+  intros Hcart Hhom.
+  unfold Noyau.
+  case (egsym _ _ _ (IdInv H)).
+  case (egsym _ _ _ (Id_gauche H _ (Fermer_inv _ _ (Fermer_id _)))).
+  case (egsym _ _ _ (Hhom _ _ (Fermer_id _) (Fermer_inv _ _ (Fermer_id _)))).
+  case (egsym _ _ _ (Hom_preserve_inv _ _ f _Hhom _ (Fermer_id _))).
+  apply conjonction.
+  apply (Fermer_ope _ _ _ (Fermer_id _) (Fermer_inv _ _ (Fermer_id _))).
+  apply (Inv_droite _ _ (Hcart _ (Fermer_id _))).
+Qed.
+
+Definition NoyauGroupeMelange (G H: Groupe) (f: Tsupp H -> Tsupp G) (Hhom: Homomorphisme _ _ f) :=
+  _SousGroupeMelange H (Noyau _ _ f) (SousNoyau _ _ f) (NoyauFermer_ope _ _ f Hhom) (NoyauFermer_inv _ _ f Hhom) (NoyauFermer_id _ _ f Hhom).
+
+Lemma Noyau_SousGroupeNormal: forall (G H: Groupe) (f: Tsupp H -> Tsupp G) 
+  (Hhom: Homomorphisme _ _ f), SousGroupeNormal _ (NoyauGroupeMelange _ _ f Hhom).
+Proof.
+  unfold SousGroupeNormal.
+  simpl. unfold Noyau.
+  intros G H f _Hhom g h Hg Nh.
+  case Nh; intros Hh Hefh.
+  apply conjonction.
+  apply Fermer_ope.
+  - apply Fermer_ope.
+  -- apply Hg.
+  -- apply Hh.
+  -  apply Fermer_inv. apply Hg.
+  - case _Hhom; intros Hcart Hhom.
+    case (egsym _ _ _ (Hhom _ _ (Fermer_ope _ _ _ Hg Hh) (Fermer_inv _ _ Hg))).
+    case (egsym _ _ _ (Hhom _ _ Hg Hh)).
+    case Hefh.
+    case Id_droite.
+  -- apply Hcart. apply Hg.
+  -- case (egsym _ _ _ (Hom_preserve_inv _ _ f _Hhom _ Hg)).
+     case Inv_droite.
+  --- apply Hcart. apply Hg.
+  --- apply egreflexion.
+Qed.
+
+Definition Image (G H: Groupe) (f: Tsupp H -> Tsupp G): Ensemble (Tsupp G) :=
+  fun x => exists h: Tsupp H, et (Supp H h) (egale _ x (f h)).
+
+Lemma ImageSousEnsemble: forall (G H: Groupe) (f: Tsupp H -> Tsupp G),
+  SousEnsemble _ (Image _ _ f) (Supp G).
+Proof.
+  unfold SousEnsemble.  
+  intros G H f x Imfx.
+  unfold Image in Imfx.
+  destruct Imfx as [h Hegxfh].
+  case Hegxfh as [Hh Hegxfh].
+
   
-  := _Groupe (Porteur G) Hsupp (Operatrice G) (Inverse G) (Elemid G)
-  HFermer_ope HFermer_inv HFermer_id
-  (fun (x y z: Porteur G) (Hx: Hsupp x) (Hy: Hsupp y) (Hz: Hsupp z)
-   => Assoc_ope G x y z (HsousG x Hx) (HsousG y Hy) (HsousG z Hz))
-  (fun (x: Porteur G) (Hx: Hsupp x) => Inv_gauche G x (HsousG x Hx))
-  (fun (x: Porteur G) (Hx: Hsupp x) => Inv_droite G x (HsousG x Hx))
-  (fun (x: Porteur G) (Hx: Hsupp x) => Id_droite G x (HsousG x Hx)).
 
+Lemma ImageFermer_ope: forall (G H: Groupe) (f: Tsupp H -> Tsupp G) (Hhom: Homomorphisme _ _ f) (x y: Tsupp G),
+  Image _ _ f x -> Image _ _ f y -> Image _ _ f (Ope _ x y).
+Proof.
+  unfold Image.  
+  intros G H f _Hhom x y Imx Imy.
+  destruct Imx as [x' Hegxfx'].
+  destruct Imy as [y' Hegyfy'].
+  exists (Ope _ x' y').
+  case Hegxfx' as [Hx' Hegxfx'].
+  case Hegyfy' as [Hy' Hegyfy'].
+  apply conjonction.
+  apply Fermer_ope.
+  - apply Hx'.
+  - apply Hy'.
+  - case _Hhom. intros Hcart Hhom.
+    case (egsym _ _ _ (Hhom x' y' Hx' Hy')).
+    case Hegxfx', Hegyfy'.
+    apply egreflexion.
+Qed.
 
+Lemma ImageFermer_inv: forall (G H: Groupe) (f: Tsupp H -> Tsupp G) (Hhom: Homomorphisme _ _ f) (x: Tsupp G),
+  Image _ _ f x -> Image _ _ f (Inv _ x).
+Proof.
+  unfold Image.
+  intros G H f _Hhom x Imx.
+  destruct Imx as [x' Hegxfx'].
+  exists (Inv _ x').
+  case Hegxfx' as [Hx' Hegxfx'].
+  apply conjonction.
+  - apply Fermer_inv. apply Hx'.
+  - case _Hhom. intros Hcart Hhom.
+    case (egsym _ _ _ (Hom_preserve_inv _ _ f _Hhom _ Hx')).
+    case Hegxfx'.
+    apply egreflexion.
+Qed.
 
-Definition SousGroupeNormal (G H: Groupe) (f: Porteur H -> Porteur G) (Homomorphisme G H f)
+Lemma ImageFermer_id: forall (G H: Groupe) (f: Tsupp H -> Tsupp G) (Hhom: Homomorphisme _ _ f),
+  Image _ _ f (Id G).
+Proof.
+  intros G H f _Hhom.
+  unfold Image.
+  exists (Id H).
+  apply conjonction.
+  - apply Fermer_id.
+  - case Hom_preserve_id. apply _Hhom. apply egreflexion.
+Qed.
 
-Definition Noyau_Supp (G H: Groupe) (f: Porteur H -> Porteur G) : Ensemble (Porteur H) :=
-  fun x => egale _ (Elemid G) (f x).
+Definition ImageSousGroupeMelange (G H: Groupe) (f: Tsupp H -> Tsupp G) :=
+  _SousGroupeMelange G (Image _ _ f) (sous) (ImageFermer_ope _ _ f Hhom) (ImageFermer_inv _ _ f Hhom) (ImageFermer_id _ _ f Hhom).
+
